removing heaps from memory and actions interfaces

ulib/experimental/Steel.Memory.fsti
@@ -20,17 +20,13 @@ module U32 = FStar.UInt32
 
 let trivial_preorder (a: Type) : Preorder.preorder a = fun _ _ -> True
 
-////////////////////////////////////////////////////////////////////////////////
-// Heap
-////////////////////////////////////////////////////////////////////////////////
 
 /// Abstract type of addresses
+
 val addr: eqtype
 
-/// Abstract type of memories
-val heap  : Type u#1
-
 /// A memory maps a reference to its associated value
+
 val array_ref (a: Type u#0) : Type u#0
 
 val length (#t: Type) (a: array_ref t) : GTot (n:U32.t)
@@ -51,18 +47,31 @@ val reference (t: Type0) : Type0
 
 val ref_address (#t: Type0) (r: reference t) : GTot addr
 
+/// The type of mem assertions
+
+val hprop : Type u#1
+
+/// Type of mem
+
+val mem : Type u#1
+
+
 /// A predicate describing non-overlapping memories
-val disjoint (m0 m1:heap) : prop
+
+val disjoint (m0 m1:mem) : prop
 
 /// disjointness is symmetric
-val disjoint_sym (m0 m1:heap)
-  : Lemma (disjoint m0 m1 <==> disjoint m1 m0)
+
+val disjoint_sym (m0 m1:mem)
+: Lemma (disjoint m0 m1 <==> disjoint m1 m0)
 
 /// disjoint memories can be combined
-val join (m0:heap) (m1:heap{disjoint m0 m1}) : heap
+
+val join (m0:mem) (m1:mem{disjoint m0 m1}) : mem
 
 /// disjointness distributes over join
-val disjoint_join (m0 m1 m2:heap)
+
+val disjoint_join (m0 m1 m2:mem)
   : Lemma (disjoint m1 m2 /\
            disjoint m0 (join m1 m2) ==>
            disjoint m0 m1 /\
@@ -70,7 +79,7 @@ val disjoint_join (m0 m1 m2:heap)
            disjoint (join m0 m1) m2 /\
            disjoint (join m0 m2) m1)
 
-val join_commutative (m0 m1:heap)
+val join_commutative (m0 m1:mem)
   : Lemma
     (requires
       disjoint m0 m1)
@@ -78,7 +87,7 @@ val join_commutative (m0 m1:heap)
       (disjoint_sym m0 m1;
        join m0 m1 == join m1 m0))
 
-val join_associative (m0 m1 m2:heap)
+val join_associative (m0 m1 m2:mem)
   : Lemma
     (requires
       disjoint m1 m2 /\
@@ -92,21 +101,22 @@ val join_associative (m0 m1 m2:heap)
 ////////////////////////////////////////////////////////////////////////////////
 
 
-/// The type of heap assertions
-val hprop : Type u#1
-/// interpreting heap assertions as memory predicates
-val interp (p:hprop) (m:heap) : prop
+/// interpreting mem assertions as memory predicates
 
-/// A common abbreviation: memories validating p
-let hheap (p:hprop) = m:heap{interp p m}
+val interp (p:hprop) (m:mem) : prop
+
 
 /// Equivalence relation on hprops is just
 /// equivalence of their interpretations
+
 let equiv (p1 p2:hprop) : prop =
   forall m. interp p1 m <==> interp p2 m
 
+
 /// All the standard connectives of separation logic
+
 val emp : hprop
+
 val pts_to_array_with_preorder
   (#t: Type0)
   (a:array_ref t)
@@ -114,6 +124,7 @@ val pts_to_array_with_preorder
   (contents:Ghost.erased (Seq.lseq t (U32.v (length a))))
   (preorder: Ghost.erased (Preorder.preorder t))
   : hprop
+
 val pts_to_ref_with_preorder
   (#t: Type0)
   (r: reference t)
@@ -121,12 +132,15 @@ val pts_to_ref_with_preorder
   (contents: Ghost.erased t)
   (preorder: Ghost.erased (Preorder.preorder t))
   : hprop
+
 val h_and (p1 p2:hprop) : hprop
 val h_or  (p1 p2:hprop) : hprop
 val star  (p1 p2:hprop) : hprop
 val wand  (p1 p2:hprop) : hprop
 val h_exists (#a:Type0) (f: (a -> hprop)) : hprop
 val h_forall (#a:Type0) (f: (a -> hprop)) : hprop
+
+type hmem (p:hprop) = m:mem{interp p m}
 
 ////////////////////////////////////////////////////////////////////////////////
 //properties of equiv
@@ -162,7 +176,7 @@ val pts_to_array_injective
   (p:permission{allows_read p})
   (c0 c1: Seq.lseq t (U32.v (length a)))
   (pre: Preorder.preorder t)
-  (m: heap)
+  (m:mem)
   : Lemma
     (requires (
       interp (pts_to_array_with_preorder a p c0 pre) m /\
@@ -193,7 +207,7 @@ val pts_to_ref_injective
   (p:permission{allows_read p})
   (c0 c1: t)
   (pre: Preorder.preorder t)
-  (m: heap)
+  (m:mem)
   : Lemma
     (requires (
       interp (pts_to_ref_with_preorder a p c0 pre) m /\
@@ -204,7 +218,7 @@ val pts_to_ref_injective
 // star
 ////////////////////////////////////////////////////////////////////////////////
 
-val intro_star (p q:hprop) (mp:hheap p) (mq:hheap q)
+val intro_star (p q:hprop) (mp:hmem p) (mq:hmem q)
   : Lemma
     (requires
       disjoint mp mq)
@@ -228,25 +242,25 @@ val star_congruence (p1 p2 p3 p4:hprop)
 ////////////////////////////////////////////////////////////////////////////////
 
 /// A low-level introduction form for wand in terms of disjoint
-val intro_wand_alt (p1 p2:hprop) (m:heap)
+val intro_wand_alt (p1 p2:hprop) (m:mem)
   : Lemma
     (requires
-      (forall (m0:hheap p1).
+      (forall (m0:hmem p1).
          disjoint m0 m ==>
          interp p2 (join m0 m)))
     (ensures
       interp (wand p1 p2) m)
 
 /// A higher-level introduction for wand as a cut
-val intro_wand (p q r:hprop) (m:hheap q)
+val intro_wand (p q r:hprop) (m:hmem q)
   : Lemma
     (requires
-      (forall (m:hheap (p `star` q)). interp r m))
+      (forall (m:hmem (p `star` q)). interp r m))
     (ensures
       interp (p `wand` r) m)
 
 /// Standard wand elimination
-val elim_wand (p1 p2:hprop) (m:heap)
+val elim_wand (p1 p2:hprop) (m:mem)
   : Lemma
     (requires
       (interp ((p1 `wand` p2) `star` p1) m))
@@ -256,31 +270,31 @@ val elim_wand (p1 p2:hprop) (m:heap)
 ////////////////////////////////////////////////////////////////////////////////
 // or
 ////////////////////////////////////////////////////////////////////////////////
-val intro_or_l (p1 p2:hprop) (m:hheap p1)
+val intro_or_l (p1 p2:hprop) (m:hmem p1)
   : Lemma (interp (h_or p1 p2) m)
 
-val intro_or_r (p1 p2:hprop) (m:hheap p2)
+val intro_or_r (p1 p2:hprop) (m:hmem p2)
   : Lemma (interp (h_or p1 p2) m)
 
 /// star can be factored out of or
-val or_star (p1 p2 p:hprop) (m:hheap ((p1 `star` p) `h_or` (p2 `star` p)))
+val or_star (p1 p2 p:hprop) (m:hmem ((p1 `star` p) `h_or` (p2 `star` p)))
   : Lemma (interp ((p1 `h_or` p2) `star` p) m)
 
 /// A standard or eliminator
-val elim_or (p1 p2 q:hprop) (m:hheap (p1 `h_or` p2))
-  : Lemma (((forall (m:hheap p1). interp q m) /\
-            (forall (m:hheap p2). interp q m)) ==> interp q m)
+val elim_or (p1 p2 q:hprop) (m:hmem (p1 `h_or` p2))
+  : Lemma (((forall (m:hmem p1). interp q m) /\
+            (forall (m:hmem p2). interp q m)) ==> interp q m)
 
 
 ////////////////////////////////////////////////////////////////////////////////
 // and
 ////////////////////////////////////////////////////////////////////////////////
-val intro_and (p1 p2:hprop) (m:heap)
+val intro_and (p1 p2:hprop) (m:mem)
   : Lemma (interp p1 m /\
            interp p2 m ==>
            interp (p1 `h_and` p2) m)
 
-val elim_and (p1 p2:hprop) (m:hheap (p1 `h_and` p2))
+val elim_and (p1 p2:hprop) (m:hmem (p1 `h_and` p2))
   : Lemma (interp p1 m /\
            interp p2 m)
 
@@ -288,10 +302,10 @@ val elim_and (p1 p2:hprop) (m:hheap (p1 `h_and` p2))
 // h_exists
 ////////////////////////////////////////////////////////////////////////////////
 
-val intro_exists (#a:_) (x:a) (p : a -> hprop) (m:hheap (p x))
+val intro_exists (#a:_) (x:a) (p : a -> hprop) (m:hmem (p x))
   : Lemma (interp (h_exists p) m)
 
-val elim_exists (#a:_) (p:a -> hprop) (q:hprop) (m:hheap (h_exists p))
+val elim_exists (#a:_) (p:a -> hprop) (q:hprop) (m:hmem (h_exists p))
   : Lemma
     ((forall (x:a). interp (p x) m ==> interp q m) ==>
      interp q m)
@@ -301,24 +315,24 @@ val elim_exists (#a:_) (p:a -> hprop) (q:hprop) (m:hheap (h_exists p))
 // h_forall
 ////////////////////////////////////////////////////////////////////////////////
 
-val intro_forall (#a:_) (p : a -> hprop) (m:heap)
+val intro_forall (#a:_) (p : a -> hprop) (m:mem)
   : Lemma ((forall x. interp (p x) m) ==> interp (h_forall p) m)
 
-val elim_forall (#a:_) (p : a -> hprop) (m:hheap (h_forall p))
+val elim_forall (#a:_) (p : a -> hprop) (m:hmem (h_forall p))
   : Lemma ((forall x. interp (p x) m) ==> interp (h_forall p) m)
 
 ////////////////////////////////////////////////////////////////////////////////
 // star
 ////////////////////////////////////////////////////////////////////////////////
 
-val affine_star (p q:hprop) (m:heap)
+val affine_star (p q:hprop) (m:mem)
   : Lemma
     (ensures (interp (p `star` q) m ==> interp p m /\ interp q m))
 
 ////////////////////////////////////////////////////////////////////////////////
 // emp
 ////////////////////////////////////////////////////////////////////////////////
-val intro_emp (m:heap)
+val intro_emp (m:mem)
   : Lemma (interp emp m)
 
 val emp_unit (p:hprop)
@@ -328,46 +342,34 @@ val emp_unit (p:hprop)
 // refinement
 ////////////////////////////////////////////////////////////////////////////////
 
-let depends_only_on (q:heap -> prop) (fp: hprop) =
-  (forall h0 h1. q h0 /\ disjoint h0 h1 ==> q (join h0 h1)) /\
-  (forall (h0:hheap fp) (h1:heap{disjoint h0 h1}). q h0 <==> q (join h0 h1))
+// let depends_only_on (q:heap -> prop) (fp: hprop) =
+//   (forall h0 h1. q h0 /\ disjoint h0 h1 ==> q (join h0 h1)) /\
+//   (forall (h0:hheap fp) (h1:heap{disjoint h0 h1}). q h0 <==> q (join h0 h1))
 
-let fp_prop fp = p:(heap -> prop){p `depends_only_on` fp}
+// let fp_prop fp = p:(heap -> prop){p `depends_only_on` fp}
 
-val weaken_depends_only_on (q:heap -> prop) (fp fp': hprop)
-  : Lemma (depends_only_on q fp ==> depends_only_on q (fp `star` fp'))
+// val weaken_depends_only_on (q:heap -> prop) (fp fp': hprop)
+//   : Lemma (depends_only_on q fp ==> depends_only_on q (fp `star` fp'))
 
-val refine (p:hprop) (q:fp_prop p) : hprop
+// val refine (p:hprop) (q:fp_prop p) : hprop
 
-val refine_equiv (p:hprop) (q:fp_prop p) (h:heap)
-  : Lemma (interp p h /\ q h <==> interp (refine p q) h)
+// val refine_equiv (p:hprop) (q:fp_prop p) (h:heap)
+//   : Lemma (interp p h /\ q h <==> interp (refine p q) h)
 
-val refine_star (p0 p1:hprop) (q:fp_prop p0)
-  : Lemma (weaken_depends_only_on q p0 p1;
-           equiv (refine (p0 `star` p1) q) (refine p0 q `star` p1))
+// val refine_star (p0 p1:hprop) (q:fp_prop p0)
+//   : Lemma (weaken_depends_only_on q p0 p1;
+//            equiv (refine (p0 `star` p1) q) (refine p0 q `star` p1))
 
-val interp_depends_only (p:hprop)
-  : Lemma (interp p `depends_only_on` p)
+// val interp_depends_only (p:hprop)
+//   : Lemma (interp p `depends_only_on` p)
 
 
-////////////////////////////////////////////////////////////////////////////////
-// Memory
-////////////////////////////////////////////////////////////////////////////////
-val mem : Type u#1
 val locks_invariant : mem -> hprop
 
-val heap_of_mem (x:mem) : heap
-
-let hmem (fp:hprop) = m:mem{interp (fp `star` locks_invariant m) (heap_of_mem m)}
+let hmem_with_inv (fp:hprop) = m:mem{interp (fp `star` locks_invariant m) m}
 
 val core_mem (m:mem) : mem
 
-val disjoint_mem (m0 m1:mem) : prop
-
-val join_mem (m0:mem) (m1:mem{disjoint_mem m0 m1}) : mem
-
-val interp_mem (hp:hprop) (m:mem) : prop
-
 let mprop (hp:hprop) = q:(mem -> prop){
-  forall (m0:mem{interp_mem hp m0}) (m1:mem{disjoint_mem m0 m1}). q m0 <==> q (join_mem m0 m1)
+  forall (m0:mem{interp hp m0}) (m1:mem{disjoint m0 m1}). q m0 <==> q (join m0 m1)
 }
